some old work in progress on atomic reduce

src/lib/poly/Kuiper.Poly.AtomicReduce.fst
@@ -14,7 +14,7 @@ let rec contributions
   (#et : Type0) {| scalar et |} {| d : has_atomic_add et |}
   (nn : nat)
   (v_done : seq bool)
-  (v_a : seq et{len v_done >= len v_a})
+  (v_a : seq et{len v_a == len v_done})
   (v_r : et) (acc : et)
 : Tot prop (decreases len v_a)
 =
@@ -30,8 +30,41 @@ let rec contributions
     else
       contributions nn tl_done tl v_r acc
 
+let rec contributions_zero 
+  (#et : Type0) {| scalar et |} {| d : has_atomic_add et |}
+  (nn : nat)
+  (v_done : seq bool)
+  (v_a : seq et{len v_a == len v_done})
+: Lemma
+  (requires v_done `Seq.equal` Seq.create (len v_done) false)
+  (ensures  contributions nn v_done v_a zero zero)
+  (decreases len v_a)
+= if len v_a = 0 then
+    ()
+  else
+    let tl = Seq.tail v_a in
+    let tl_done = Seq.tail v_done in
+    contributions_zero nn tl_done tl
+
+// let rec contributions_split
+//   (#et : Type0) {| scalar et |} {| d : has_atomic_add et |}
+//   (nn : nat)
+//   (v_done_0 v_done_1 : seq bool)
+//   (v_a_0 v_a_1 : seq et{len v_a == len v_done})
+//   (v_r : et) (acc : et)
+
+let contrib
+  (#et : Type0) {| scalar et |} {| d : has_atomic_add et |}
+  (nn : nat)
+  (v_done : seq bool)
+  (v_a : seq et{len v_done == len v_a})
+  (v_r : et) (acc : et)
+: slprop
+= pure (contributions nn v_done v_a v_r acc)
+
 let inv_p
   (#et : Type0) {| scalar et |} {| d : has_atomic_add et |}
+  (f:perm)
   (nn: nat)
   (a: gpu_array et nn)
   (v_a: seq et)
@@ -40,15 +73,16 @@ let inv_p
 =
   // pure (len done == nn) **
   exists* (v_done:
-    seq bool {len v_done >= len done /\ len v_done >= len v_a})
+    seq bool {len v_done == len done /\ len v_done == len v_a})
     v_r.
-    ((a |-> v_a) ** (r |-> v_r) **
-    bigstar 0 (len done) (fun i -> gref_pts_to (done @! i) #0.5R (v_done @! i))) **
-    pure (contributions nn v_done v_a v_r zero)
+    (gpu_pts_to_array a #f v_a) ** (r |-> v_r) **
+    bigstar 0 (len done) (fun i -> gref_pts_to (done @! i) #0.5R (v_done @! i)) **
+    contrib nn v_done v_a v_r zero
 
 unfold
 let kpre
   (#et : Type0) {| scalar et |} {| d : has_atomic_add et |}
+  (f:perm)
   (nn: nat)
   (a : gpu_array et nn)
   (v_a : seq et)
@@ -58,11 +92,12 @@ let kpre
   (tid : natlt nn)
 =
   gref_pts_to (done @! tid) #0.5R false **
-  inv i (inv_p nn a v_a r done)
+  inv i (inv_p f nn a v_a r done)
 
 unfold
 let kpost
   (#et : Type0) {| scalar et |} {| d : has_atomic_add et |}
+  (f:perm)
   (nn: nat)
   (a : gpu_array et nn)
   (v_a : seq et)
@@ -72,7 +107,7 @@ let kpost
   (tid : natlt nn)
 =
   gref_pts_to (done @! tid) #0.5R true **
-  inv i (inv_p nn a v_a r done)
+  inv i (inv_p f nn a v_a r done)
 
 ghost
 fn bigstar_ghost_upd_lemma
@@ -82,48 +117,107 @@ fn bigstar_ghost_upd_lemma
   requires
     bigstar 0 (len done) (fun i -> gref_pts_to (done @! i) #0.5R (v_done @! i)) **
     gref_pts_to (done @! tid) #0.5R false
-  // returns
-  //   v_done' : (v_done' : seq bool{len v_done' >= len done})
   ensures
     bigstar 0 (len done) (fun i -> gref_pts_to (done @! i) #0.5R ((Seq.upd v_done tid true) @! i)) **
     gref_pts_to (done @! tid) #0.5R true
 {
-  admit();
+  open Pulse.Lib.GhostReference;
+  bigstar_extract 0 (len done) _ tid;
+  gather (done @! tid);
+  (done @! tid) := true;
+  share (done @! tid);
+  bigstar_rw_congr 0 tid 
+    (fun i -> gref_pts_to (done @! i) #0.5R (v_done  @! i))
+    (fun i -> gref_pts_to (done @! i) #0.5R ((Seq.upd v_done tid true) @! i)) (fun _ -> ());
+  bigstar_rw_congr (tid + 1) (len done)
+    (fun i -> gref_pts_to (done @! i) #0.5R (v_done  @! i))
+    (fun i -> gref_pts_to (done @! i) #0.5R ((Seq.upd v_done tid true) @! i)) (fun _ -> ());
+  bigstar_compose 0 (len done) (fun i -> gref_pts_to (done @! i) #0.5R ((Seq.upd v_done tid true) @! i)) tid;
 }
 
-assume
-val contributions_lemma
+let contributions_lemma
   (#et : Type0) {| scalar et |} {| d : has_atomic_add et |}
   (nn: nat)
   (v_done : seq bool)
-  (v_a : seq et{len v_done >= len v_a})
+  (v_a : seq et{len v_done == len v_a})
   (v_r : et) (acc : et)
   (tid : nat{tid < len v_a})
-  : Lemma (requires contributions nn v_done v_a v_r acc /\ v_done @! tid == false)
-          (ensures  contributions nn (Seq.upd v_done tid true) v_a (d.pure_op v_r (v_a @! tid)) acc)
-          [SMTPat (contributions nn (Seq.upd v_done tid true) v_a (d.pure_op v_r (v_a @! tid)) acc)]
+: Lemma
+  (requires contributions nn v_done v_a v_r acc /\ v_done @! tid == false)
+  (ensures  contributions nn (Seq.upd v_done tid true) v_a (d.pure_op (v_a @! tid) v_r) acc)
+  // [SMTPat (contributions nn (Seq.upd v_done tid true) v_a (d.pure_op (v_a @! tid) v_r) acc)]
+= admit()
+
+ghost
+fn vdone_bid_false
+  (#v_done : seq bool)
+  (tid : nat)
+  (done : seq (gref bool) {
+     len v_done >= len done /\ len done > tid 
+    })
+requires
+    bigstar 0 (len done) (fun i -> gref_pts_to (done @! i) #0.5R (v_done @! i)) **
+    gref_pts_to (done @! tid) #0.5R false
+ensures
+    bigstar 0 (len done) (fun i -> gref_pts_to (done @! i) #0.5R (v_done @! i)) **
+    gref_pts_to (done @! tid) #0.5R false **
+    pure (v_done @! tid == false)
+{
+  bigstar_extract 0 (len done) _ tid;
+  Pulse.Lib.GhostReference.pts_to_injective_eq (done @! tid);
+  bigstar_compose 0 (len done) (fun i -> gref_pts_to (done @! i) #0.5R (v_done @! i)) tid;
+}
+
+ghost
+fn upd_contrib 
+  (#et : Type0) {| scalar et |} {| d : has_atomic_add et |}
+  (#nn: nat)
+  (v_done : seq bool)
+  (v_a : seq et{len v_done == len v_a})
+  (#v_r : et) 
+  (#acc : et)
+  (tid : nat{tid < len v_a})
+  (done : seq (gref bool) {
+     len v_done == len done /\ len done > tid 
+    })
+requires
+  contrib nn v_done v_a v_r acc **
+  bigstar 0 (len done) (fun i -> gref_pts_to (done @! i) #0.5R (v_done @! i)) **
+  gref_pts_to (done @! tid) #0.5R false
+ensures 
+  contrib nn (Seq.upd v_done tid true) v_a (d.pure_op (v_a @! tid) v_r) acc **
+  bigstar 0 (len done) (fun i -> gref_pts_to (done @! i) #0.5R ((Seq.upd v_done tid true) @! i)) **
+  gref_pts_to (done @! tid) #0.5R true
+{
+  vdone_bid_false #v_done tid done;
+  unfold (contrib nn v_done v_a v_r acc);
+  contributions_lemma nn v_done v_a v_r acc tid;
+  fold (contrib nn (Seq.upd v_done tid true) v_a (d.pure_op (v_a @! tid) v_r) acc);
+  bigstar_ghost_upd_lemma done v_done tid;
+}
+
 
 inline_for_extraction noextract
 fn kf
-  (#et : Type0) {| scalar et |} {| d : has_atomic_add et |}
+  (#et : Type0) {| sc_et : scalar et |} {| d : has_atomic_add et |}
+  (#f:perm)
   (#nn: SZ.t)
   (a : gpu_array et (SZ.v nn))
   (#v_a : erased (seq et))
   (r : gpu_ref et)
-  (done : erased (seq (gref bool)){len done == reveal nn})
+  (done : erased (seq (gref bool)){len done == reveal nn /\ len v_a == len done})
   (i : iname)
   (bid : szlt (SZ.v nn))
   ()
   requires
     gpu **
-    kpre (SZ.v nn) a v_a r done i bid **
+    kpre f (SZ.v nn) a v_a r done i bid **
     block_id (SZ.v nn) bid
   ensures
     gpu **
-    kpost (SZ.v nn) a v_a r done i bid **
+    kpost f (SZ.v nn) a v_a r done i bid **
     block_id (SZ.v nn) bid
 {
-  assume (pure (len v_a == reveal nn));
   later_credit_buy 1;
   later_credit_buy 1;
   (* Read array at idx *)
@@ -134,34 +228,35 @@ fn kf
         gpu **
         block_id (SZ.v nn) bid **
         gref_pts_to (done @! bid) #0.5R false **
-        later (inv_p (SZ.v nn) a v_a r done) **
+        later (inv_p f (SZ.v nn) a v_a r done) **
         pure (v == v_a @! SZ.v bid) **
         later_credit 1
     {
       later_elim _;
-      unfold (inv_p (SZ.v nn) a v_a r done);
+      unfold (inv_p f (SZ.v nn) a v_a r done);
       let rr = gpu_array_read #et #(SZ.v nn) #0 #(SZ.v nn) a bid;
-      fold (inv_p (SZ.v nn) a v_a r done);
-      later_intro (inv_p (SZ.v nn) a v_a r done);
+      fold (inv_p f (SZ.v nn) a v_a r done);
+      later_intro (inv_p f (SZ.v nn) a v_a r done);
       rr
     };
   (* Fetch and add into result cell. *)
   with_invariants i
   {
     later_elim _;
-    unfold (inv_p (SZ.v nn) a v_a r done);
+    unfold (inv_p f (SZ.v nn) a v_a r done);
+    with nn' v_done v_a' v_r acc.
+      assert (contrib #et #sc_et #d nn' v_done v_a' v_r acc);
     let _ = atomic_add r v;
-    bigstar_ghost_upd_lemma done _ _ ;
-    rewrite each SZ.v bid as bid;
-    assume (pure False); (* FIXME *)
-    fold (inv_p (SZ.v nn) a v_a r done);
-    later_intro (inv_p (SZ.v nn) a v_a r done);
+    upd_contrib v_done v_a bid done; //need to explicitly instantate v_done and v_a
+    fold (inv_p f (SZ.v nn) a v_a r done);
+    later_intro (inv_p f (SZ.v nn) a v_a r done);
   }
 }
 
 ghost
 fn done_lemma
   (#et : Type0) {| scalar et |} {| d : has_atomic_add et |}
+  (f:perm)
   (nn: erased nat)
   (a : gpu_array et nn)
   (r : gpu_ref et)
@@ -169,95 +264,295 @@ fn done_lemma
   (i : iname)
   (v_a : erased (seq et))
   requires
-    gpu **
-    bigstar 0 nn (fun tid -> kpost  nn a v_a r done i tid)
+    bigstar 0 nn (fun tid -> kpost f nn a v_a r done i tid)
   ensures
-    gpu **
     (r |-> Kuiper.Seq.Common.seq_fold_left d.pure_op zero v_a) **
-    (a |-> v_a)
+    (gpu_pts_to_array a #f v_a)
 {
   admit();
 }
 
+[@@erasable]
+noeq
+type i_done (n:nat) = {
+  i: iname;
+  done: seq (gref bool);
+  pf: squash (len done == n)
+}
+instance non_informative_i_done (n:nat)
+: Pulse.Lib.NonInformative.non_informative (i_done n) = {
+  reveal = (fun r -> Ghost.reveal r) <: Pulse.Lib.NonInformative.revealer (i_done n);
+}
+
+let iname_of #n (x: i_done n) : iname = x.i
+let refs_of #n (x: i_done n) : erased (seq (gref bool)) = x.done
 
 ghost
-fn setup
+fn rec bigstar_share
+    (l0 l1: int)
+    (m :nat)
+    (n :nat {m <= n})
+    (f g h: (i:nat {m <= i /\ i < n} -> slprop))
+    (share_i : 
+      (i:nat {m <= i /\ i < n} -> stt_ghost unit emp_inames (requires f i) (ensures fun _ -> g i ** h i)))
+requires bigstar m n f
+ensures bigstar #l0 m n g ** bigstar #l1 m n h
+decreases (n - m)
+{
+  if (m = n)
+  {
+    rewrite bigstar m n f as bigstar m m f;
+    bigstar_zs_elim #_ #_ #f;
+    bigstar_zs_intro m g;
+    bigstar_zs_intro m h;
+    bigstar_ext 0 l0 m n h h;
+    bigstar_ext 0 l1 m n g g;
+    rewrite bigstar m m h as bigstar #l0 m n h;
+    rewrite bigstar m m g as bigstar #l1 m n g;
+  }
+  else
+  {
+    ghost
+    fn share_i' (i:nat {m + 1 <= i /\ i < n})
+    requires f i 
+    ensures g i ** h i
+    {
+      share_i i;
+    };
+    bigstar_split #0 m n f (m + 1);
+    rewrite bigstar m n f 
+    as bigstar m (m + 1) f ** bigstar (m + 1) n f;
+    bigstar_share l0 l1 (m + 1) n f g h share_i';
+    bigstar_single_elim #0 #m #f;
+    share_i m;
+    bigstar_single_intro #l0 m g;
+    bigstar_single_intro #l1 m h;
+    bigstar_paste #l0 #m #n (m + 1) #g;
+    bigstar_paste #l1 #m #n (m + 1) #h;
+  }
+}
+
+
+ghost
+fn rec alloc_refs (n:nat)
+requires emp
+returns refs : (s : seq (gref bool) { len s == n })
+ensures bigstar 0 n (fun i -> gref_pts_to (refs @! i) false)
+decreases n
+{
+  open Pulse.Lib.BigStar;
+  if (n=0)
+  {
+    let refs = Seq.empty #(gref bool);
+    bigstar_zs_intro 0 (fun i -> gref_pts_to (refs @! i) false);
+    rewrite 
+       bigstar 0 0 (fun i -> gref_pts_to (refs @! i) false)
+    as bigstar 0 n (fun i -> gref_pts_to (refs @! i) false);
+    refs
+  }
+  else
+  {
+    let refs = alloc_refs (n-1);
+    let r = Pulse.Lib.GhostReference.alloc false;
+    let refs' = Seq.snoc refs r;
+    bigstar_rw_congr #0 0 (n - 1)
+      (fun i -> gref_pts_to (refs @! i) false) 
+      (fun i -> gref_pts_to (refs' @! i) false) //NS: needed to be very explicit
+      (fun i -> () <: squash (gref_pts_to (refs @! i) false == gref_pts_to (refs' @! i) false)); 
+    rewrite gref_pts_to r false as gref_pts_to (refs' @! (n-1)) false;
+    //NS: needed to be very careful about the bound var type of the lambda
+    bigstar_single_intro (n - 1) (fun (i:nat { 0 <= i /\ i < n }) -> gref_pts_to (refs' @! i) false);
+    //NS: so that i can use it in paste
+    bigstar_paste #_ #0 #(n - 1 + 1) (n - 1);
+    rewrite each (n - 1 + 1) as n;
+    refs'
+  }
+}
+
+ghost
+fn intro_contrib_zero #et {| scalar et |} {| d : has_atomic_add et |}
+      (nn: nat) (v_a: seq et { nn == len v_a }) //(v_r: et { v_r == zero })
+requires emp
+returns v_done : (s:seq bool { len s == nn /\ s == Seq.create nn false })
+ensures contrib nn v_done v_a zero zero
+{
+  let v_done = Seq.create nn false;
+  contributions_zero nn v_done v_a;
+  fold (contrib nn v_done v_a zero zero);
+  v_done
+}
+
+ghost
+fn relabel_bigstar #l0 #l1 (m:nat) (n:nat {m <= n}) (f: (i:nat {m <= i /\ i < n} -> slprop))
+requires bigstar #l0 m n f
+ensures bigstar #l1 m n f
+{
+  bigstar_extensionality_lem l0 l1 m n f f (fun _ -> slprop_equiv_refl _);
+  rewrite bigstar #l0 m n f
+       as bigstar #l1 m n f;
+}
+
+ghost
+fn pre_setup
   (#et : Type0) {| scalar et |} {| d : has_atomic_add et |}
+  (#f:perm)
   (n : sz)
   (a : gpu_array et n)
-  (#f : perm)
   (#v_a : erased (seq et))
   (r : gpu_ref et)
   requires
     cpu **
     gpu_pts_to_array a #f v_a **
     (r |-> zero #et) **
-    pure (SZ.v n <= 1024)
+    pure (SZ.v n <= 1024 /\ len v_a == SZ.v n)
   returns
-    i_done : iname & erased (seq (gref bool))
+    i_done : i_done (SZ.v n)
   ensures
-    (match i_done with | (i, done) ->
-    cpu
-    ** W.with_pure (len done == SZ.v n) (fun _ ->
-       bigstar 0 (SZ.v n) (fun tid ->
-        gref_pts_to (done @! tid) #0.5R false **
-        inv i (inv_p (SZ.v n) a v_a r done))
-    ))
+    cpu **
+    bigstar 0 (SZ.v n) (fun tid -> gref_pts_to (refs_of i_done @! tid) #0.5R false) **
+    inv (iname_of i_done) (inv_p f (SZ.v n) a v_a r (refs_of i_done))
 {
-  admit();
+  let refs = alloc_refs (SZ.v n);
+  ghost
+  fn share_ref_i (i:nat { 0 <= i /\ i < SZ.v n })
+  requires gref_pts_to (refs @! i) false
+  ensures gref_pts_to (refs @! i) #0.5R false ** gref_pts_to (refs @! i) #0.5R false
+  {
+    Pulse.Lib.GhostReference.share (refs @! i);
+  };
+  bigstar_share 0 1 0 (SZ.v n) 
+    (fun i -> gref_pts_to (refs @! i) false) 
+    (fun i -> gref_pts_to (refs @! i) #0.5R false) 
+    (fun i -> gref_pts_to (refs @! i) #0.5R false)
+    share_ref_i;
+  let v_done = intro_contrib_zero n v_a;
+  rewrite each (SZ.v n) as (len refs);
+  bigstar_rw_congr #0 0 (len refs) 
+    (fun i -> gref_pts_to (refs @! i) #0.5R false)
+    (fun i -> gref_pts_to (refs @! i) #0.5R (v_done @! i))
+    (fun i -> ()); //<: squash (gref_pts_to (refs @! i) #0.5R false == gref_pts_to (refs @! i) #0.5R (v_done @! i)));
+  fold (inv_p f (SZ.v n) a v_a r refs);
+  let i = new_invariant (inv_p f (SZ.v n) a v_a r refs);
+  relabel_bigstar #1 #0 0 (len refs) _;
+  let result : i_done (SZ.v n) = { i = i; done = refs; pf = () };
+  rewrite each (len refs) as (SZ.v n);
+  rewrite each refs as (refs_of result);
+  rewrite each i as (iname_of result);
+  result
+}
+
+ghost
+fn rec replicate 
+    (p:slprop)
+    (m:nat)
+    (n:nat { m <= n })
+    (dup: (unit -> stt_ghost unit emp_inames (requires p) (ensures fun _ -> p ** p)))
+requires p
+ensures p ** bigstar m n (fun i -> p)
+decreases (n - m)
+{
+  open Pulse.Lib.BigStar;
+  if (m = n)
+  {
+    bigstar_zs_intro m (fun i -> p);
+    rewrite bigstar m m (fun i -> p)
+         as bigstar m n (fun i -> p);
+  }
+  else
+  {
+    dup (); 
+    replicate p (m + 1) n dup;
+    bigstar_single_intro m 
+      (fun (i:nat { m <= i /\ i < n }) -> p);
+    bigstar_paste #_ #m #n (m + 1) 
+      #(fun (i:nat { m <= i /\ i < n }) -> p);
+  }
+}
+
+ghost
+fn setup 
+  (#et : Type0) {| scalar et |} {| d : has_atomic_add et |}
+  (#f:perm)
+  (n : szp{n < max_blocks})
+  (a : gpu_array et n)
+  (#v_a : erased (seq et))
+  (r : gpu_ref et)
+  (done : erased (seq (gref bool)){len done == SZ.v n})
+  (i : iname)
+  ()
+requires
+  bigstar 0 (SZ.v n) (fun tid -> gref_pts_to (done @! tid) #0.5R false) **
+  inv i (inv_p f (SZ.v n) a v_a r done)
+ensures
+  (forall+ (bid: natlt n). kpre f n a v_a r done i bid)  **
+  emp
+{
+  ghost fn duplicate ()
+  requires
+    inv i (inv_p f (SZ.v n) a v_a r done)
+  ensures
+    inv i (inv_p f (SZ.v n) a v_a r done) **
+    inv i (inv_p f (SZ.v n) a v_a r done)
+  {
+    dup_inv _ _;
+  };
+  replicate _ 0 (SZ.v n) duplicate;
+  bigstar_zip 0 (SZ.v n)
+      (fun i -> gref_pts_to (done @! i) #0.5R false)
+      (fun _ -> inv i (inv_p f (SZ.v n) a v_a r done));
+  rewrite 
+    bigstar 0 (SZ.v n) (fun tid -> gref_pts_to (done @! tid) #0.5R false **
+      inv i (inv_p f (SZ.v n) a v_a r done))
+  as bigstar 0 (SZ.v n) (fun tid -> kpre f n a v_a r done i tid);
+  forevery_fromstar #(natlt n) (fun tid -> kpre f n a v_a r done i tid);
+  drop_ (inv i _);
 }
 
 ghost
 fn teardown
   (#et : Type0) {| scalar et |} {| d : has_atomic_add et |}
+  (f:perm)
   (n : sz)
   (a : gpu_array et n)
-  (#f : perm)
   (#v_a : erased (seq et))
   (r : gpu_ref et)
-  (i : iname)
   (done : lseq (gref bool) (SZ.v n))
-  // returns
-  //   i_done : erased (iname & erased (seq (gref bool)))
+  (i : iname)
+  ()
   requires
-    pure (len done == SZ.v n) **
-    bigstar 0 (SZ.v n) (fun tid ->
-     gref_pts_to (done @! tid) #0.5R true **
-     inv i (inv_p (SZ.v n) a v_a r done))
+    (forall+ (bid: natlt n). kpost f n a v_a r done i bid) **
+    emp
   ensures
     gpu_pts_to_array a #f v_a **
-    (r |-> Kuiper.Seq.Common.seq_fold_left d.pure_op zero v_a) **
-    pure (SZ.v n <= 1024)
+    (r |-> Kuiper.Seq.Common.seq_fold_left d.pure_op zero v_a) 
 {
-  admit();
+  forevery_tonat (SZ.v n) (fun tid -> kpost f n a v_a r done i tid);
+  done_lemma f (SZ.v n) a r done i v_a;
 }
 
 inline_for_extraction noextract
 let kdesc
   (#et : Type0) {| scalar et |} {| d : has_atomic_add et |}
+  (#f:perm)
   (n : szp{n < max_blocks})
   (a : gpu_array et n)
-  (#f : perm)
   (#v_a : erased (seq et))
   (r : gpu_ref et)
   (#r0 : erased et)
-  (* FIXME: these two arguments should be created by the setup
-     and passed to each block. We should extend the kernel_desc
-     to allow for that. *)
-  (done : erased (seq (gref bool)){len done == SZ.v n})
+  (done : erased (seq (gref bool)){len done == SZ.v n /\ len v_a == len done})
   (i : iname)
 : kernel_desc
-    (gpu_pts_to_array a #f v_a **
-      (r |-> r0))
+    (bigstar 0 (SZ.v n) (fun tid -> gref_pts_to (done @! tid) #0.5R false) **
+    inv i (inv_p f (SZ.v n) a v_a r done))
     (gpu_pts_to_array a #f v_a **
       (r |-> Kuiper.Seq.Common.seq_fold_left d.pure_op zero v_a))
  = {
   nblk = n;
   f = kf a #v_a r done i;
-  setup = magic();
-  teardown = magic();
-  kpre  = kpre  n a v_a r done i;
-  kpost = kpost n a v_a r done i;
+  setup=setup n a r done i;
+  teardown = teardown f n a #v_a r done i;
+  kpre  = kpre f n a v_a r done i;
+  kpost = kpost f n a v_a r done i;
   frame = emp;
 } <: kernel_desc_m_1 _ _
 
@@ -280,6 +575,7 @@ fn reduce
     gpu_pts_to_array a #f v_a **
     pure (r == Kuiper.Seq.Common.seq_fold_left d.pure_op zero v_a)
 {
+  gpu_pts_to_ref a;
   let mut r = zero #et #_;
   let gr = gpu_alloc0 #et ();
   Kuiper.Ref.gpu_memcpy_host_to_device #et #_ gr r;
@@ -289,34 +585,8 @@ fn reduce
 
   assert (pure (n < max_blocks));
 
-  // let i_done = setup n a gr;
-  // let i = (i_done)._1;
-  // let done : erased (seq (gref bool)) = hide (reveal (i_done._2));
-  // rewrite each i_done as (i, done) by (tadmit());
-  // New fancy syntax, does not extract
-  // let Mktuple2 i done = setup n a gr;
-  // The problem is essentially https://github.com/FStarLang/pulse/issues/93.
-  // The match is over a (Pulse) non-informative type, a pair of iname and erased (seq (gref bool)).
-  // It gets erased to unit, but the patterns do not, so the match is ill-typed and krml complains.
-
-  // W.elim_with_pure (len done == SZ.v n) _;
-
-  let done = magic #(erased (seq (gref bool))) ();
-  let i    = magic #iname ();
-  assume (pure (len done == SZ.v n));
-  // (done : erased (seq (gref bool)){len done == SZ.v n})
-
-  launch_sync (kdesc n a #f #v_a gr #(zero #et) done i);
-
-  // launch_kernel_n_blocks n
-  //   #(kpre  (SZ.v n) a v_a gr done i)
-  //   #(kpost (SZ.v n) a v_a gr done i)
-  //   (fun tid -> k (hide n) a gr done i v_a tid);
-
-  // forevery_tostar #(natlt (SZ.v n))
-  //   (kpost (SZ.v n) a v_a gr done i);
-
-  // teardown n a #f #v_a gr i done;
+  let i_done = pre_setup n a gr;
+  launch_sync (kdesc n a #v_a gr #(zero #et) (refs_of i_done) (iname_of i_done));
 
   Kuiper.Ref.gpu_memcpy_device_to_host r gr #_ #_ #_;
 
